Foundation/Propositional/Logic/Extension.lean
@@ -1,0 +1,42 @@
+import Foundation.Propositional.Hilbert.WellKnown
+import Foundation.Propositional.Kripke.Logic.Int
+
+
+namespace LO.Propositional
+
+namespace Logic
+
+class Superintuitionistic (L : Logic) where
+  subset_Int : Logic.Int ⊆ L
+  mdp_closed {φ ψ} : φ ➝ ψ ∈ L → φ ∈ L → ψ ∈ L
+  subst_closed {φ} : φ ∈ L → ∀ s, φ⟦s⟧ ∈ L
+
+end Logic
+
+
+namespace Hilbert
+
+open Entailment
+
+variable {H : Hilbert ℕ}
+
+protected instance superintuitionistic [H.HasEFQ] : (H.logic).Superintuitionistic where
+  subset_Int := by
+    intro φ hφ;
+    induction hφ using Hilbert.Deduction.rec! with
+    | maxm h =>
+      rcases (by simpa using h) with ⟨s, rfl⟩; simp;
+    | mdp ihφψ ihφ => exact mdp! ihφψ ihφ;
+    | _ => simp;
+  mdp_closed := by
+    intro φ ψ hφψ hφ;
+    exact hφψ ⨀ hφ;
+  subst_closed := by
+    intro φ hφ s;
+    exact Hilbert.Deduction.subst! s hφ;
+
+end Hilbert
+
+instance : (Logic.Int).Superintuitionistic := Hilbert.superintuitionistic
+
+end LO.Propositional
